Reorganised theories so that termination is defined in terms of weakest precondition, and linked this to total correctness Hoare logic

UTP/ITree_THoare.thy
@@ -4,11 +4,8 @@ theory ITree_THoare
   imports ITree_Hoare
 begin
 
-definition prog_term_under :: "('e, 's) htree \<Rightarrow> ('s \<Rightarrow> bool) \<Rightarrow> bool"
-  where "prog_term_under C P = (\<forall> s. P s \<longrightarrow> terminates (C s))"
-
 definition thoare_triple :: "('s \<Rightarrow> bool) \<Rightarrow> ('e, 's) htree \<Rightarrow> ('s \<Rightarrow> bool) \<Rightarrow> bool" where
-"thoare_triple P S Q = (hoare_triple P S Q \<and> prog_term_under S P)"
+"thoare_triple P S Q = (hoare_triple P S Q \<and> `P \<longrightarrow> pre S`)"
 
 syntax
   "_thoare"          :: "logic \<Rightarrow> logic \<Rightarrow> logic \<Rightarrow> logic" ("H[_]/ _/ [_]")
@@ -19,18 +16,19 @@ translations
 lemma thoare_then_hoare: "H[P] C [Q] \<Longrightarrow> H{P} C {Q}"
   by (simp add: thoare_triple_def)
 
-lemma thoareI: "\<lbrakk> H{P} C {Q}; prog_term_under C (P)\<^sub>e \<rbrakk> \<Longrightarrow> H[P] C [Q]"
+lemma thoareI: "\<lbrakk> H{P} C {Q}; `P \<longrightarrow> pre C` \<rbrakk> \<Longrightarrow> H[P] C [Q]"
   by (simp add: thoare_triple_def)
 
 lemma thl_conseq:
   assumes "H[P\<^sub>2] S [Q\<^sub>2]" "`P\<^sub>1 \<longrightarrow> P\<^sub>2`" "`Q\<^sub>2 \<longrightarrow> Q\<^sub>1`"
   shows "H[P\<^sub>1] S [Q\<^sub>1]"
   using assms 
-  by (simp add: thoare_triple_def hoare_alt_def prog_term_under_def)
+  by (simp add: thoare_triple_def hoare_alt_def)
      (expr_auto, blast)
 
 lemma thl_skip: "H[P] Skip [P]"
-  by (auto simp add: thoare_triple_def prog_term_under_def hoare_alt_def Skip_def terminates_Ret)
+  by (auto simp add: thoare_triple_def hoare_alt_def terminates_Ret Skip_def)
+     (metis (no_types, lifting) SEXP_def Skip_def tautI wp_Skip)
 
 lemma thl_skip': 
   assumes "`P \<longrightarrow> Q`"
@@ -38,11 +36,11 @@ lemma thl_skip':
   by (meson assms hl_skip' thl_skip thoare_triple_def)
 
 lemma thl_seq: "\<lbrakk> H[P] S\<^sub>1 [Q]; H[Q] S\<^sub>2 [R] \<rbrakk> \<Longrightarrow> H[P] S\<^sub>1 ;; S\<^sub>2 [R]"
-  by (auto simp add: thoare_triple_def hl_seq prog_term_under_def)
-     (auto intro!: terminates_bind simp add: seq_itree_def kleisli_comp_def hoare_alt_def retvals_def)
+  by (auto simp add: thoare_triple_def hl_seq wp)
+     (simp add: hoare_alt_def wp_alt_def seq_itree_def kleisli_comp_def, expr_auto, meson)
 
 lemma thl_assigns: "H[\<sigma> \<dagger> P] \<langle>\<sigma>\<rangle>\<^sub>a [P]"
-  by (metis assigns_def hoare_assigns prog_term_under_def terminates_Ret thoare_triple_def)
+  by (simp add: thoare_triple_def hoare_assigns wp, subst_eval)
 
 lemma thl_assign: "H[P\<lbrakk>e/x\<rbrakk>] x := e [P]"
   by (rule thl_assigns)
@@ -50,9 +48,7 @@ lemma thl_assign: "H[P\<lbrakk>e/x\<rbrakk>] x := e [P]"
 lemma thl_cond [hoare_safe]:
   assumes "H[B \<and> P] S [Q]" "H[\<not>B \<and> P] T [Q]"
   shows "H[P] if B then S else T fi [Q]"
-  using assms
-  by (auto simp add: thoare_triple_def hl_cond)
-     (simp add: cond_itree_def prog_term_under_def)
+  using assms by (simp add: thoare_triple_def hl_cond wp taut_def)
 
 lemma thl_while [hoare_safe]:
   fixes V :: "'s \<Rightarrow> 'a::wellorder"
@@ -64,14 +60,15 @@ proof -
   hence partial: "\<^bold>{P\<^bold>} while B do S od \<^bold>{\<not> B \<and> P\<^bold>}"
     by (rule hoare_while_partial)
   from assms have S_term: "\<And> s. \<lbrakk> B s; P s \<rbrakk> \<Longrightarrow> terminates (S s)"
-    by (simp add: thoare_triple_def SEXP_def prog_term_under_def)  
-
-  from assms have wS_term: "prog_term_under (while B do S od) P"
-    unfolding thoare_triple_def hoare_alt_def prog_term_under_def
-    by (auto intro!: terminates_iterate_wellorder_variant[of B P S V] simp add: SEXP_def)
-
+    by (simp add: thoare_triple_def pre_terminates, simp add: hoare_alt_def taut_def)  
+  from assms have wS_term: "`P \<longrightarrow> pre (while B do S od)`"
+    by (auto simp add: pre_terminates taut_def thoare_triple_def hoare_alt_def) 
+       (auto intro!: terminates_iterate_wellorder_variant[of B P S V] simp add: SEXP_def)
   show ?thesis
-    by (metis SEXP_def partial thoareI wS_term)
+    using partial thoareI wS_term by fastforce
 qed
+
+lemma thl_via_wlp_wp: "H[P] S [Q] = `P \<longrightarrow> (wlp S Q \<and> pre S)`"
+  by (simp add: thoare_triple_def hl_via_wlp, expr_auto)
 
 end
